exercicio 1 feito

1.dfy
@@ -1,11 +1,14 @@
 /*                                      Cumulative Sums over Arrays                                        */
 
-
-/*_________________________________________________________________________________________________________*/
+/*
+    Daniel Cavalheiro   57869
+    Pedro Nunes         57854
+*/
 
 
 
 //(a)
+
 function sum(a: array<int>, i: int, j: int): int
     reads a
     requires 0 <= i <= j <= a.Length
@@ -16,7 +19,9 @@ function sum(a: array<int>, i: int, j: int): int
 }
 
 
+
 //(b)
+
 method query(a: array<int>, i: int, j: int) returns (res:int)
     requires 0 <= i <= j <= a.Length
     ensures res == sum(a, i, j)
@@ -35,3 +40,31 @@ method query(a: array<int>, i: int, j: int) returns (res:int)
 }
 
 
+
+//(c)
+
+predicate is_prefix_sum_for (a: array<int>, c: array<int>)
+    requires a.Length + 1 == c.Length
+    requires c[0] == 0
+    reads c, a
+{
+    forall i: int :: 0 <= i < a.Length ==> c[i+1] == c[i] + a[i]
+}
+
+lemma aux(a: array<int>, c: array<int>, i: int, j: int)
+    requires 0 <= i <= j <= a.Length
+    requires a.Length + 1 == c.Length
+    requires c[0] == 0
+    requires is_prefix_sum_for(a, c)
+    decreases j - i
+    ensures forall k: int :: i <= k <= j ==> sum(a, i, k) + sum(a, k, j) == c[k] - c[i] + c[j] - c[k] //sum(a, i, j) == c[j] - c[i]
+
+method queryFast(a: array<int>, c: array<int>, i: int, j: int) returns (r: int)
+    requires a.Length + 1 == c.Length && c[0] == 0
+    requires 0 <= i <= j <= a.Length
+    requires is_prefix_sum_for(a,c)  
+    ensures r == sum(a, i, j)
+{   
+    aux(a, c, i, j);
+    r := c[j] - c[i];    
+}
